Verification of computePath

src/verification/dafny/astar_navfnplanner.dfy
@@ -1,17 +1,18 @@
 datatype Point = Point(row: int, col: int)
+datatype RealPoint = RealPoint(row: real, col: real)
 datatype Pose = Pose(pos: Point)
 datatype CostMap = CostMap(value: Point -> real, numRows: nat, numCols: nat)
 datatype RealInf = Real(r: real) | Infinity
 
 
-type Path = seq<Pose>
+type Path = seq<RealPoint>
 type PotentialMap = seq<seq<RealInf>>
 
 const obstacleCost: real := 254.0
 const mapCost: real := 50.0
 
 
-predicate method open(costMap: CostMap, row: int, col: int)
+predicate method Open(costMap: CostMap, row: int, col: int)
 {
   costMap.value(Point(row, col))  < obstacleCost
 }
@@ -25,7 +26,7 @@ predicate ValidPotentialMap(pot: PotentialMap, costMap: CostMap)
 {
   PotentialMapHasDimensions(pot, costMap.numRows, costMap.numCols)
   && forall i, j | 0 <= i < costMap.numRows && 0 <= j < costMap.numCols ::
-    pot[i][j].Real? ==> open(costMap, i, j)
+    pot[i][j].Real? ==> Open(costMap, i, j)
 }
 
 predicate ValidCostMap(costMap: CostMap)
@@ -50,6 +51,21 @@ predicate Adjacent(p1: Pose, p2: Pose, costMap: CostMap)
   AdjacentHorizontal(p1, p2) || AdjacentVertical(p1, p2)
 }
 
+function method AdjacentOf(p: Point): seq<Point>
+{
+  [Point(p.row - 1, p.col - 1),
+   Point(p.row - 1, p.col),
+   Point(p.row - 1, p.col + 1),
+   Point(p.row, p.col - 1),
+   Point(p.row, p.col + 1),
+   Point(p.row + 1, p.col - 1),
+   Point(p.row + 1, p.col),
+   Point(p.row + 1, p.col + 1)
+  ]
+}
+
+
+
 predicate HasSomeAdjacentReal(p: Pose, pot: PotentialMap, numRows: nat, numCols: nat)
   requires PotentialMapHasDimensions(pot, numRows, numCols)
   requires 0 <= p.pos.row < numRows && 0 <= p.pos.col < numCols
@@ -70,19 +86,32 @@ predicate ValidQueue(queue: seq<Pose>, pot: PotentialMap, costMap: CostMap)
     && HasSomeAdjacentReal(p, pot, costMap.numRows, costMap.numCols)
 }
 
-method AStar(start: Pose, goal: Pose, costMap: CostMap, numIterations: nat) returns (path: Path)
+method AStar(start: Pose, goal: Pose, costMap: CostMap, numIterations: nat) returns (error: bool, path: Path)
   requires 0 <= start.pos.row < costMap.numRows && 0 <= start.pos.col < costMap.numCols
   requires 0 <= goal.pos.row < costMap.numRows && 0 <= goal.pos.col < costMap.numCols
-  requires open(costMap, goal.pos.row, goal.pos.col)
+  requires Open(costMap, goal.pos.row, goal.pos.col)
   requires ValidCostMap(costMap)
+  ensures !error ==>
+    |path| >= 1
+    && path[0] == RealPoint(start.pos.row as real, start.pos.col as real)
+    && path[|path| - 1] == RealPoint(goal.pos.row as real, goal.pos.col as real)
+    && forall p | p in path :: Open(costMap, ClosestPoint(p).row, ClosestPoint(p).col)
+
 {
   var pot := BuildInitialPotentialMap(costMap.numRows, costMap.numCols, goal.pos.row, goal.pos.col);
   var initialThreshold := EuclidDistance(start.pos, goal.pos);
   initialThreshold := initialThreshold + obstacleCost;
   var current := InitCurrentQueue(goal, pot, costMap);
 
-  var pot' := AStarIteration(start, goal, costMap, pot, current, [], [], initialThreshold, numIterations);
-  path := ComputePath(start, goal, pot', costMap.numRows, costMap.numCols);
+  var pot': PotentialMap := AStarIteration(start, goal, costMap, pot, current, [], [], initialThreshold, numIterations);
+  ghost var closestPath: seq<Point>;
+  if (pot'[start.pos.row][start.pos.col].Real?) {
+    error, path, closestPath := ComputePath(start.pos, goal.pos, pot', numIterations, costMap.numRows, costMap.numCols);
+    assert !error ==> forall p | p in path :: pot'[ClosestPoint(p).row][ClosestPoint(p).col].Real?;
+    assert !error ==> forall p | p in path :: Open(costMap, ClosestPoint(p).row, ClosestPoint(p).col);
+  } else {
+    error := true;
+  }
 }
 
 method AStarIteration(start: Pose, goal: Pose,
@@ -106,7 +135,7 @@ method AStarIteration(start: Pose, goal: Pose,
   }
 
   if (|current| > 0) {
-    if (!open(costMap, current[0].pos.row, current[0].pos.col)) {
+    if (!Open(costMap, current[0].pos.row, current[0].pos.col)) {
       pot' := AStarIteration(start, goal, costMap, pot, current[1..], next, excess, threshold, numIterations);
       return;
     } else {
@@ -141,7 +170,7 @@ method BuildInitialPotentialMap(numRows: nat, numCols: nat, initRow: nat,  initC
 {
   var i := 0;
   var j := 0;
-  
+
   p := seq(numRows, i => seq(numCols, j => Infinity));
   p := p[initRow := p[initRow][initCol := Real(0.0)]];
 }
@@ -154,13 +183,13 @@ method InitCurrentQueue(p: Pose, ghost pot: PotentialMap, costMap: CostMap) retu
   ensures ValidQueue(current, pot, costMap)
 {
   var p1l :=
-    if (p.pos.row > 0 && open(costMap, p.pos.row - 1, p.pos.col)) then [Pose(Point(p.pos.row - 1, p.pos.col))] else [];
+    if (p.pos.row > 0 && Open(costMap, p.pos.row - 1, p.pos.col)) then [Pose(Point(p.pos.row - 1, p.pos.col))] else [];
   var p2l :=
-    if (p.pos.row + 1 < costMap.numRows && open(costMap, p.pos.row + 1, p.pos.col)) then [Pose(Point(p.pos.row + 1, p.pos.col))] else [];
+    if (p.pos.row + 1 < costMap.numRows && Open(costMap, p.pos.row + 1, p.pos.col)) then [Pose(Point(p.pos.row + 1, p.pos.col))] else [];
   var p3l :=
-    if (p.pos.col > 0 && open(costMap, p.pos.row, p.pos.col - 1)) then [Pose(Point(p.pos.row, p.pos.col - 1))] else [];
+    if (p.pos.col > 0 && Open(costMap, p.pos.row, p.pos.col - 1)) then [Pose(Point(p.pos.row, p.pos.col - 1))] else [];
   var p4l :=
-    if (p.pos.col + 1 < costMap.numCols && open(costMap, p.pos.row, p.pos.col + 1)) then [Pose(Point(p.pos.row, p.pos.col + 1))] else [];
+    if (p.pos.col + 1 < costMap.numCols && Open(costMap, p.pos.row, p.pos.col + 1)) then [Pose(Point(p.pos.row, p.pos.col + 1))] else [];
 
   current := p1l + p2l + p3l + p4l;
 }
@@ -170,7 +199,7 @@ method UpdatePotential(pot: PotentialMap, p: Pose, goal: Pose, costMap: CostMap,
   requires ValidCostMap(costMap)
   requires 0 <= p.pos.row < costMap.numRows && 0 <= p.pos.col < costMap.numCols
   requires min.Real?
-  requires open(costMap, p.pos.row, p.pos.col)
+  requires Open(costMap, p.pos.row, p.pos.col)
   ensures ValidPotentialMap(pot', costMap)
   ensures forall i, j | 0 <= i < costMap.numRows && 0 <= j < costMap.numCols ::
     pot[i][j].Real? ==> pot'[i][j].Real?
@@ -199,28 +228,28 @@ method TraverseNeighbors(p: Pose, start: Pose, costMap: CostMap, pot: PotentialM
   ensures ValidQueue(next', pot, costMap) && ValidQueue(excess', pot, costMap)
 {
   var p1l, p1r: seq<Pose>;
-  if (p.pos.row > 0 && open(costMap, p.pos.row - 1, p.pos.col)) {
+  if (p.pos.row > 0 && Open(costMap, p.pos.row - 1, p.pos.col)) {
     p1l, p1r := TraverseNeighbor(p, Pose(Point(p.pos.row - 1, p.pos.col)), start, costMap, pot, threshold);
   } else {
     p1l := []; p1r := [];
   }
 
   var p2l, p2r: seq<Pose>;
-  if (p.pos.row < costMap.numRows - 1 && open(costMap, p.pos.row + 1, p.pos.col)) {
+  if (p.pos.row < costMap.numRows - 1 && Open(costMap, p.pos.row + 1, p.pos.col)) {
     p2l, p2r := TraverseNeighbor(p, Pose(Point(p.pos.row + 1, p.pos.col)), start, costMap, pot, threshold);
   } else {
     p2l := []; p2r := [];
   }
 
   var p3l, p3r: seq<Pose>;
-  if (p.pos.col > 0 && open(costMap, p.pos.row, p.pos.col - 1)) {
+  if (p.pos.col > 0 && Open(costMap, p.pos.row, p.pos.col - 1)) {
     p3l, p3r := TraverseNeighbor(p, Pose(Point(p.pos.row, p.pos.col - 1)), start, costMap, pot, threshold);
   } else {
     p3l := []; p3r := [];
   }
 
   var p4l, p4r: seq<Pose>;
-  if (p.pos.col < costMap.numCols - 1 && open(costMap, p.pos.row, p.pos.col + 1)) {
+  if (p.pos.col < costMap.numCols - 1 && Open(costMap, p.pos.row, p.pos.col + 1)) {
     p4l, p4r := TraverseNeighbor(p, Pose(Point(p.pos.row, p.pos.col + 1)), start, costMap, pot, threshold);
   } else {
     p4l := []; p4r := [];
@@ -253,16 +282,30 @@ method TraverseNeighbor(p: Pose, newP: Pose, start: Pose, costMap: CostMap, pot:
   }
 }
 
-method ComputePath(start: Pose, goal: Pose, pot: PotentialMap, numRows: nat, numCols: nat) returns (p: Path)
 
-function method Abs(x: int): int {
+function method AbsInt(x: int): int {
   if (x >= 0) then x else -x
 }
 
+function method AbsReal(x: real): real {
+  if (x >= 0.0) then x else -x
+}
+
+function method SignReal(x: real): real {
+  if (x > 0.0) then 1.0
+  else if (x < 0.0) then -1.0
+  else 0.0
+}
+
+function method ClosestPoint(p: RealPoint): Point {
+  Point((p.row + 0.5).Floor, (p.col + 0.5).Floor)
+}
+
+
 
 method EuclidDistance(p1: Point, p2: Point) returns (d: real) {
-  var diffRows := Abs(p1.row - p2.row);
-  var diffCols := Abs(p1.col - p2.col);
+  var diffRows := AbsInt(p1.row - p2.row);
+  var diffCols := AbsInt(p1.col - p2.col);
   d := (diffRows * diffRows + diffCols * diffCols) as real; // TODO: sqrt?
 }
 
@@ -302,8 +345,145 @@ predicate method GreaterThan(x1: RealInf, x2: RealInf)
   x1.Infinity? || (x2.Real? && x1.r > x2.r)
 }
 
+predicate method GreaterThanOrEqual(x1: RealInf, x2: RealInf)
+{
+  x1.Infinity? || (x1.Real? && x2.Real? && x1.r >= x2.r)
+}
+
+
 function method Minus(x1: RealInf, x2: RealInf): RealInf
   requires x2.Real?
 {
   if (x1.Infinity?) then Infinity else Real(x1.r - x2.r)
 }
+
+predicate method AllFree(p: Point, potentialMap: PotentialMap, ghost numRows: nat, ghost numCols: nat)
+  requires |potentialMap| == numRows
+  requires forall x | x in potentialMap :: |x| == numCols
+{
+  if (|potentialMap| == 0) then
+    false
+  else
+    0 < p.row < |potentialMap| - 1 && 0 < p.col < |potentialMap[0]| - 1
+    && forall adj | adj in AdjacentOf(p) :: potentialMap[adj.row][adj.col].Real?
+}
+
+
+method ComputePath(start: Point, goal: Point, potentialMap: PotentialMap, numSteps: nat, numRows: nat, numCols: nat)
+  returns (error: bool, path: seq<RealPoint>, ghost closest: seq<Point>)
+  requires PotentialMapHasDimensions(potentialMap, numRows, numCols)
+  requires 0 <= start.row < numRows && 0 <= start.col < numCols
+  requires potentialMap[start.row][start.col].Real?
+  ensures !error ==>
+            |path| == |closest|
+            && |path| >= 1
+            && path[0] == RealPoint(start.row as real, start.col as real)
+            && path[|path| - 1] == RealPoint(goal.row as real, goal.col as real)
+            && forall i | 0 <= i < |path| :: ClosestPoint(path[i]) == closest[i]
+            && forall i | 0 <= i < |closest| :: 0 <= closest[i].row < numRows && 0 <= closest[i].col < numCols && potentialMap[closest[i].row][closest[i].col].Real?
+{
+  var i := numSteps;
+  var p: RealPoint := RealPoint(start.row as real, start.col as real);
+  ghost var cl := ClosestPoint(p);
+  assert cl == start;
+  path := [p];
+  closest := [cl];
+  error := false;
+  while (i > 0 && !error && ClosestPoint(p) != goal)
+    decreases !error, i
+    invariant !error ==> 0 <= cl.row < numRows && 0 <= cl.col < numCols
+    invariant !error ==> cl == ClosestPoint(p)
+    invariant !error ==> potentialMap[cl.row][cl.col].Real?
+    invariant |path| == |closest|
+    invariant |path| > 0
+    invariant path[0] == RealPoint(start.row as real, start.col as real)
+    invariant forall i | 0 <= i < |path| :: ClosestPoint(path[i]) == closest[i]
+    invariant forall i | 0 <= i < |closest| :: 0 <= closest[i].row < numRows && 0 <= closest[i].col < numCols &&
+        potentialMap[closest[i].row][closest[i].col].Real?
+  {
+    error, p, cl := NextMove(p, cl, potentialMap, numRows, numCols);
+    if (!error) {
+      path := path + [p];
+      closest := closest + [cl];
+      i := i - 1;
+    }
+  }
+
+  if (error || i == 0) {
+    error := true;
+  } else {
+    error := false;
+    path := path + [RealPoint(goal.row as real, goal.col as real)];
+    closest := closest + [goal];
+  }
+}
+
+method NextMove(p: RealPoint, ghost closest: Point, potentialMap: PotentialMap, numRows: nat, numCols: nat)
+  returns (error: bool, p': RealPoint, ghost closest': Point)
+  requires PotentialMapHasDimensions(potentialMap, numRows, numCols)
+  requires 0 <= closest.row < numRows && 0 <= closest.col < numCols
+  requires closest == ClosestPoint(p)
+  requires potentialMap[closest.row][closest.col].Real?
+  ensures !error ==> closest' == ClosestPoint(p')
+  ensures !error ==> 0 <= closest'.row < numRows && 0 <= closest'.col < numCols
+  ensures !error ==> potentialMap[closest'.row][closest'.col].Real?
+{
+  var cp := ClosestPoint(p);
+  assert cp == closest;
+  if (AllFree(cp, potentialMap, numRows, numCols)) {
+    var drow: real := *;
+    var dcol: real := *;
+
+    if (AbsReal(drow) > 1.0) {
+      drow := SignReal(drow);
+    }
+    if (AbsReal(dcol) > 1.0) {
+      dcol := SignReal(dcol);
+    }
+    assert -1.0 <= drow <= 1.0;
+    assert -1.0 <= dcol <= 1.0;
+
+    p' := RealPoint(p.row + drow, p.col + dcol);
+    closest' := ClosestPoint(p');
+    error := false;
+
+    assert 0 <= closest'.row < numRows;
+    assert 0 <= closest'.col < numCols;
+
+    assert potentialMap[closest'.row][closest'.col].Real?;
+  } else {
+    p' := p;
+    closest' := ClosestPoint(p');
+
+    var adjs := AdjacentOf(cp);
+    var i := 0;
+    var min_idx := 0;
+
+    while (i < |adjs|)
+      invariant 0 <= i <= |adjs|
+      invariant 0 <= min_idx < |adjs|
+      invariant forall j | 0 <= j < i ::
+        (adjs[j].row < 0 || adjs[j].row >= numRows || adjs[j].col < 0 || adjs[j].col >= numCols ||
+         adjs[min_idx].row < 0 || adjs[min_idx].row >= numRows || adjs[min_idx].col < 0 || adjs[min_idx].col >= numCols ||
+        GreaterThanOrEqual(potentialMap[adjs[j].row][adjs[j].col], potentialMap[adjs[min_idx].row][adjs[min_idx].col]))
+    {
+      if (0 <= adjs[i].row < numRows && 0 <= adjs[i].col < numCols &&
+          0 <= adjs[min_idx].row < numRows && 0 <= adjs[min_idx].col < numCols &&
+          !GreaterThanOrEqual(potentialMap[adjs[i].row][adjs[i].col], potentialMap[adjs[min_idx].row][adjs[min_idx].col])) {
+        min_idx := i;
+      }
+      i := i + 1;
+    }
+
+    if (adjs[min_idx].row < 0 || adjs[min_idx].row >= numRows || adjs[min_idx].col < 0 || adjs[min_idx].col >= numCols ||
+      potentialMap[adjs[min_idx].row][adjs[min_idx].col].Infinity?) {
+      error :=  true;
+    } else {
+      error := false;
+      p' := RealPoint(adjs[min_idx].row as real, adjs[min_idx].col as real);
+      closest' := ClosestPoint(p');
+      assert potentialMap[closest'.row][closest'.col].Real?;
+    }
+  }
+}
+
